lib/Utils/FunctionalFP.v
@@ -1,0 +1,48 @@
+
+Section FunctionalFP.
+  Variable (A: Type).
+  Variable (f: A -> A).
+
+  Fixpoint iter (n: nat) (a: A) : A := 
+    match n with 
+    | 0 => a
+    | S n' => f (iter n' a)
+    end.
+
+  Variable (eqb: A -> A -> bool).
+
+  Fixpoint iter' (n: nat) (a: A) : A := 
+    match n with 
+    | 0 => a
+    | S n' => 
+      let nxt := f a in 
+      if eqb nxt a then nxt else f (iter' n' a)
+    end.
+
+  Variable (eqb_sound: forall a a', eqb a a' = true <-> a = a').
+
+  Lemma iter_iter' : 
+    forall n a,
+    iter n a = iter' n a.
+  Proof.
+    intros.
+    induction n.
+    - simpl. reflexivity.
+    - unfold iter; fold iter.
+      unfold iter'; fold iter'.
+      pose proof (@eqb_sound (f a) a).
+      destruct (eqb _ _) eqn:?.
+      + destruct H as [H' _].
+        erewrite H'; trivial.
+        erewrite IHn.
+
+        destruct n; simpl iter'; [eapply H'; trivial|].
+
+        specialize (@eqb_sound (f a) a).
+        destruct eqb_sound as [_ H''].
+        erewrite H''; erewrite H'; trivial.
+        eapply H'; trivial.
+      + erewrite IHn; trivial.
+  Qed.
+
+End FunctionalFP.
